%Imo19952Mo
Legyen $x=\frac{1}{a},\ y=\frac{1}{b},\ z=\frac{1}{c}.$ Ekkor a bizonyítandó az:
$$
\frac{x^{3}}{\frac{1}{y}+\frac{1}{z}}+
\frac{y^{3}}{\frac{1}{z}+\frac{1}{x}}+
\frac{z^{3}}{\frac{1}{x}+\frac{1}{y}} =
\frac{x^{2}}{y+z}+
\frac{y^{2}}{z+x}+
\frac{z^{2}}{x+y}=(*)
$$
alakot ölti. Tovább becsülhetjük $(*)$-ot a \nameref{FolEng1Fa}-val:
$$
(*) \ge \frac{\Gzjel{x+y+z}^{2}}{(y+z)+(z+x)+(x+y)} = 
   \frac{1}{2}(x+y+z) \ge \frac{1}{2} 3\Gzjel{xyz}^{\frac{1}{3}}=\frac{3}{2}, 
$$
ahol használtuk még \nameref{AlapAMGMFa}-et és $xyz=1$-et.
